Logic/Predicate/Semantics.lean
@@ -66,8 +66,8 @@ lemma extendStructure_rel
   simp[Language.Hom.extendStructure]
   refine ⟨by intros h; rcases h with ⟨r₁', e, h⟩; rcases injr e; exact h, by intros h; refine ⟨r₁, rfl, h⟩⟩
 
-class Eq (L : Language.{u}) [L.HasEq] (M : Type w) [s : Structure L M] where
-  eq : ∀ a b, s.rel Language.HasEq.eq ![a, b] ↔ a = b
+class Eq (L : Language.{u}) [L.Eq] (M : Type w) [s : Structure L M] where
+  eq : ∀ a b, s.rel Language.Eq.eq ![a, b] ↔ a = b
 
 attribute [simp] Eq.eq
 
